Refactor WP rules and begin proving load acquire rule

src/high/protocol.v
@@ -1,8 +1,8 @@
 From iris.base_logic.lib Require Import own ghost_map.
 From iris.proofmode Require Import reduction monpred tactics.
+From iris_named_props Require Import named_props.
 
 From self.high Require Import dprop resources post_crash_modality monpred_simpl.
-(* From self.high Require Import proofmode wpc_proofmode. *)
 From self.lang Require Import lang.
 
 
@@ -18,31 +18,26 @@ Class LocationProtocol `{AbstractState ST, nvmFixedG Σ} (ϕ : loc_pred ST) := {
   bumper : ST → ST;
   bumper_mono :> Proper ((⊑@{ST}) ==> (⊑))%signature bumper;
   phi_condition :
-    (⊢ ∀ (hD : nvmDeltaG Σ) s v, ϕ s v hD -∗ <PCF> hD', ϕ (bumper s) v hD' : dProp Σ)%I
+    (⊢ ∀ (hD : nvmDeltaG Σ) s v,
+      ϕ s v hD -∗ <PCF> hD', ϕ (bumper s) v hD' : dProp Σ)%I
 }.
 
 (** [know_protocol] represents the knowledge that a location is associated with a
 specific protocol. It's defined simply using more "primitive" assertions. *)
 Definition know_protocol `{AbstractState ST, nvmFixedG Σ, nvmDeltaG Σ}
            ℓ ϕ `{!LocationProtocol ϕ} : dProp Σ :=
-  ⎡ know_pred ℓ ϕ ⎤ ∗
-  ⎡ know_preorder_loc ℓ (⊑@{ST}) ⎤ ∗
-  ⎡ know_bumper ℓ bumper ⎤%I.
+  "#knowPred" ∷ ⎡ know_pred ℓ ϕ ⎤ ∗
+  "#knowPreorder" ∷ ⎡ know_preorder_loc ℓ (⊑@{ST}) ⎤ ∗
+  "#knowBumper" ∷ ⎡ know_bumper ℓ bumper ⎤%I.
 
 Section protocol.
-  Context `{nvmFixedG Σ, nvmDeltaG Σ}.
-  Context `{AbstractState ST}.
-
-  (* Context (ϕ : loc_pred (Σ := Σ) ST) (ℓ : loc). *)
-  (* Context `{!LocationProtocol ϕ}. *)
+  Context `{nvmFixedG Σ, nvmDeltaG Σ, AbstractState ST}.
 
   Lemma post_crash_know_protocol ℓ ϕ `{!LocationProtocol ϕ} :
     know_protocol ℓ ϕ -∗ <PC> hD, or_lost ℓ (know_protocol ℓ ϕ).
   Proof.
-    iIntros "(a & b & c)".
-    iCrash.
-    rewrite /know_protocol.
-    rewrite -?or_lost_sep.
+    iIntros "(? & ? & ?)". iCrash.
+    rewrite /know_protocol. rewrite -?or_lost_sep.
     iFrame.
   Qed.
 
@@ -50,6 +45,8 @@ Section protocol.
     IntoCrash
       (know_protocol ℓ ϕ)%I
       (λ hG', or_lost ℓ (know_protocol ℓ ϕ))%I.
-  Proof. rewrite /IntoCrash. iIntros "P". by iApply post_crash_know_protocol. Qed.
+  Proof.
+    rewrite /IntoCrash. iIntros "P". by iApply post_crash_know_protocol.
+  Qed.
 
 End protocol.
