src/high/weakestpre_at.v
@@ -1,0 +1,395 @@
+(* Weakest precondition rules for atomic locations. *)
+
+From stdpp Require Import gmap.
+From iris.program_logic Require weakestpre.
+
+From stdpp Require Import countable numbers gmap.
+From iris Require Import invariants.
+From iris.proofmode Require Import tactics monpred.
+From iris.algebra Require Import gmap gset excl auth.
+From iris.program_logic Require weakestpre.
+From iris.heap_lang Require Import locations.
+From iris_named_props Require Import named_props.
+
+From self Require Export extra ipm_tactics.
+From self.high Require Export dprop.
+From self Require Export view.
+From self Require Export lang.
+From self.base Require Import tactics.
+From self.base Require Import primitive_laws.
+From self.lang Require Import syntax.
+From self.high Require Import resources crash_weakestpre lifted_modalities
+     monpred_simpl modalities protocol.
+
+Section wp_at_rules.
+  Context `{AbstractState ST}.
+  Context `{!nvmFixedG Σ, hG : nvmDeltaG Σ}.
+
+  Implicit Types (ℓ : loc) (s : ST) (ϕ : ST → val → nvmDeltaG Σ → dProp Σ).
+
+  (** * Shared points-to predicate *)
+
+  Lemma predicate_holds_phi_decode ϕ s encS (encϕ : predO) v TV :
+    decode encS = Some s →
+    (encϕ ≡ encode_predicate ϕ)%I -∗
+    (encoded_predicate_holds encϕ encS v TV ∗-∗ ϕ s v _ TV).
+  Proof.
+    iIntros (eq') "predsEquiv".
+    iSplit.
+    - iDestruct 1 as (P') "[%eq PH]".
+      iDestruct (discrete_fun_equivI with "predsEquiv") as "HI".
+      iDestruct ("HI" $! encS) as "HIP". (* iClear "HI". *)
+      iEval (rewrite discrete_fun_equivI) in "HIP".
+      iDestruct ("HIP" $! v) as "HI". (* iClear "HIP". *)
+      rewrite /encode_predicate.
+      rewrite eq'.
+      simpl.
+      rewrite option_equivI.
+      rewrite eq.
+      iEval (setoid_rewrite discrete_fun_equivI) in "HI".
+      iSpecialize ("HI" $! hG).
+      by iRewrite "HI" in "PH".
+    - iIntros "phi".
+      rewrite /encoded_predicate_holds.
+      do 2 iEval (setoid_rewrite discrete_fun_equivI) in "predsEquiv".
+      iSpecialize ("predsEquiv" $! encS v).
+      rewrite /encode_predicate. rewrite eq'.
+      simpl.
+      destruct (encϕ encS v); rewrite option_equivI; last done.
+      iExists _. iSplit; first done.
+      iEval (setoid_rewrite discrete_fun_equivI) in "predsEquiv".
+      iSpecialize ("predsEquiv" $! hG).
+      by iRewrite "predsEquiv".
+  Qed.
+
+  Lemma msg_persisted_views_eq'
+        (ℓ : loc) (hists : gmap loc (gmap time message))
+        (hist : gmap time message) (msg : message)
+        (sharedLocs : gset loc) (t : time) :
+    map_Forall
+      (λ _ : loc,
+        map_Forall
+          (λ _ msg, msg_persist_view msg = msg_persisted_after_view msg))
+      (restrict sharedLocs hists) →
+    ℓ ∈ sharedLocs →
+    hists !! ℓ = Some hist →
+    hist !! t = Some msg →
+    msg.(msg_persist_view) = msg.(msg_persisted_after_view).
+  Proof.
+  Admitted.
+
+  Lemma msg_persisted_views_eq
+        (ℓ : loc) (hists : gmap loc (gmap time (message * positive)))
+        (hist : gmap time (message * positive)) (msg : message)
+        (sharedLocs : gset loc) (t : time) (s' : positive) :
+    map_Forall
+      (λ _ : loc,
+        map_Forall
+          (λ _ '(msg, _), msg_persist_view msg = msg_persisted_after_view msg))
+      (restrict sharedLocs hists) →
+    hists !! ℓ = Some hist →
+    hist !! t = Some (msg, s') →
+    own shared_locs_name (● (sharedLocs : gsetUR loc)) -∗
+    own shared_locs_name (◯ {[ℓ]}) -∗
+    ⌜msg.(msg_persist_view) = msg.(msg_persisted_after_view)⌝.
+  Proof.
+    iIntros (m look look') "A B".
+    iDestruct (location_sets_singleton_included with "A B") as %V.
+    iPureIntro.
+    assert (restrict sharedLocs hists !! ℓ = Some hist) as look2.
+    - apply restrict_lookup_Some. done.
+    - setoid_rewrite map_Forall_lookup in m.
+      specialize (m ℓ hist look2).
+      setoid_rewrite map_Forall_lookup in m.
+      specialize (m t (msg, s') look').
+      simpl in m.
+      done.
+  Qed.
+
+  Lemma wp_load_shared ℓ s Q ϕ `{!LocationProtocol ϕ} positive E :
+    {{{
+      "knowProt" ∷ know_protocol ℓ ϕ ∗
+      "isSharedLoc" ∷ ⎡ is_shared_loc ℓ ⎤ ∗
+      "storeLB" ∷ know_store_lb ℓ s ∗
+      "pToQ" ∷ <obj> (∀ s' v, ⌜ s ⊑ s' ⌝ -∗ ϕ s' v _ -∗ Q s' v ∗ ϕ s' v _)
+    }}}
+      !{acq} #ℓ @ positive; E
+    {{{ s' v, RET v;
+      "storeLB" ∷ know_store_lb ℓ s' ∗
+      post_fence (Q s' v) }}}.
+  Proof.
+    intros Φ.
+    iStartProof (iProp _). iIntros (TV).
+    iNamed 1.
+    iDestruct "knowProt" as "(knowPred & _ & _)".
+    iNamed "storeLB".
+    (* We unfold the WP. *)
+    iIntros (TV' incl) "Φpost".
+    rewrite wp_eq /wp_def wpc_eq.
+    iIntros ([[SV PV] BV] incl2) "#val".
+    monPred_simpl.
+    iApply program_logic.crash_weakestpre.wp_wpc.
+
+    iApply wp_extra_state_interp_fupd.
+    { done. }
+    { (* Try and simplify this with lemmas/automation. *)
+      clear.
+      intros ??????? [Ki [??] [??] ? ? step].
+      subst.
+      simpl in *.
+      induction Ki using rev_ind.
+      { simpl in *. subst. inv_impure_thread_step; try done.
+        rewrite list_fmap_singleton.
+        subst.
+        congruence. }
+      move: H.
+      rewrite fill_app.
+      simpl.
+      destruct x; try done.
+      simpl.
+      rewrite /thread_fill_item.
+      simpl.
+      inversion 1.
+      simpl in *.
+      rewrite -nvm_fill_fill in H2.
+      simpl in *.
+      destruct Ki using rev_ind; try done.
+      { simpl in *. subst. inv_impure_thread_step; try done. }
+      simpl in *.
+      rewrite fill_app in H2.
+      simpl in *.
+      destruct x; try done. }
+    (* We open [interp]. *)
+    iNamed 1.
+
+    (* _Before_ we load the points-to predicate we deal with the predicate ϕ. We
+    do this before such that the later that arrises is stripped off when we take
+    the step. *)
+    iDestruct (own_all_preds_pred with "predicates knowPred")
+      as (pred predsLook) "#predsEquiv".
+
+    (* We need to get the points-to predicate for [ℓ] which is is inside
+    [interp].  We want to look up the points-to predicate in [ptsMap]. To this
+    end, we combine our fragment of the history with the authorative element. *)
+    iDestruct (
+        own_frag_history_agree_singleton with "history knowFragHist") as %look.
+    destruct look as (absHist & enc & absHistLook & lookTS & decodeEnc).
+
+    iDestruct (
+        location_sets_singleton_included with "sharedLocs isSharedLoc"
+      ) as %ℓSh.
+    iDestruct (big_sepM_lookup_acc with "predsHold") as "[predMap predsHold]".
+    { done. }
+    iDestruct "predMap" as
+        (pred' physHist physHistLook predsLook') "predMap".
+    assert (pred = pred') as <-. { apply (inj Some). rewrite -predsLook. done. }
+    clear predsLook'.
+
+    (* We can now get the points-to predicate and execute the load. *)
+    iDestruct (big_sepM_lookup_acc with "ptsMap") as "[pts ptsMap]"; first done.
+    (* iApply wp_fupd. *)
+    iApply (wp_load_acquire (extra := {| extra_state_interp := True |})
+             with "[$pts $val]").
+    iIntros "!>" (t' v' SV' PV' _PV') "(%look & %gt & #val' & pts)".
+
+    rewrite /store_view.
+    iDestruct ("ptsMap" with "pts") as "ptsMap".
+    iFrame "val'".
+
+    (* We show that [PV'] is equal to [_PV']. *)
+    assert (PV' = _PV') as <-.
+    { eapply msg_persisted_views_eq' in mapShared; try done. done. }
+
+    assert (tS ≤ t') as lte.
+    { destruct TV as [[??]?].
+      destruct TV' as [[??]?].
+      etrans; first done.
+      etrans; last done.
+      rewrite /store_view /=.
+      f_equiv.
+      etrans. apply incl. apply incl2. }
+
+    iDestruct (big_sepM2_dom with "predMap") as %domEq.
+    assert (is_Some (absHist !! t')) as (encSL & HI).
+    { apply elem_of_dom. rewrite <- domEq. apply elem_of_dom. naive_solver. }
+    iDestruct (big_sepM2_lookup_acc with "predMap") as "[predHolds predMap]";
+      [done|done| ].
+    simpl.
+
+    (* The loaded state must be greater than [s]. *)
+    iDestruct (big_sepM2_lookup_l with "ordered")
+      as (order) "[%ordersLook %increasingMap]".
+    { apply absHistLook. }
+    iDestruct (orders_lookup with "allOrders order") as %orderEq;
+      first apply ordersLook.
+    epose proof (increasingMap tS t' (encode s) encSL) as hihi.
+    assert (order enc encSL) as orderRelated.
+    { destruct (le_lt_or_eq _ _ lte) as [le|tSEq].
+      - eapply increasingMap.
+        * apply le.
+        * subst. done.
+        * done.
+      - (* We can conclude that [enc] is equal to [t']. *)
+        assert (enc = encSL) as ->.
+        2: { rewrite orderEq. rewrite /encode_relation.
+             rewrite decodeEnc. simpl. done. }
+        congruence. }
+    rewrite orderEq in orderRelated.
+    epose proof (encode_relation_related _ _ _ orderRelated)
+      as (? & sL & eqX & decodeS' & s3InclS').
+    assert (x = s') as -> by congruence.
+
+    iDestruct (predicate_holds_phi_decode with "predsEquiv predHolds") as "PH";
+      first done.
+    iSpecialize ("pToQ" $! (SV', PV', ∅) sL v').
+    monPred_simpl.
+    iEval (setoid_rewrite monPred_at_wand) in "pToQ".
+    iDestruct ("pToQ" $! (SV', PV', ∅) with "[//] [%] [//] PH") as "[Q phi]".
+    { etrans; done. }
+    (* Reinsert into the predicate map. *)
+    iDestruct ("predMap" with "[phi]") as "predMap".
+    { iFrame "%".
+      iApply (predicate_holds_phi_decode with "predsEquiv phi").
+      done. }
+    (* Reinsert into the map. *)
+    iDestruct ("predsHold" with "[predMap]") as "predsHold".
+    { iExists _, _. naive_solver. }
+
+    (* Note: This allocation was commented out. Do we need it? *)
+    (* iMod (own_full_history_alloc_frag with "history") as "[history histS]"; try done. *)
+    (* iModIntro. *)
+    (* We re-establish [interp]. *)
+    iSplitR "ptsMap allOrders ordered predsHold history predicates
+             crashedAt sharedLocs allBumpers bumpMono predPostCrash"; last first.
+    { repeat iExists _. iModIntro. iFrameNamed. }
+    iSplit. { iPureIntro. repeat split; try done; apply view_le_l. }
+    iSpecialize ("Φpost" $! sL v').
+    monPred_simpl.
+    iApply "Φpost".
+    { iPureIntro.
+      etrans. eassumption.
+      repeat split; try done; try apply view_le_l. }
+    (* The thread view we started with [TV] is smaller than the view we ended
+    with. *)
+    assert (TV ⊑ (SV ⊔ SV', PV, BV ⊔ PV')).
+    { do 2 (etrans; first done). repeat split; auto using view_le_l. }
+    iSplitR "Q".
+    - iFrameNamed.
+      iExists t', sL.
+      iFrame "∗#".
+      iSplit; first done.
+      (* FIXME: Intuitively the lhs. should be included in because we read [t']
+      and a write includes its own timestamp. But, we don't remember this fact,
+      yet. *)
+      admit.
+    - simpl.
+      rewrite /store_view /flush_view /=.
+      iApply monPred_mono; last iApply "Q".
+      repeat split.
+      * apply view_le_r.
+      * rewrite assoc. apply view_le_r.
+      * apply view_empty_least.
+  Admitted.
+
+  Lemma wp_store_rel ℓ v s1 s2 ϕ `{!LocationProtocol ϕ} positive E :
+    {{{
+      "knowProt" ∷ know_protocol ℓ ϕ ∗
+      "isSharedLoc" ∷ ⎡ is_shared_loc ℓ ⎤ ∗
+      "storeLB" ∷ know_store_lb ℓ s1 ∗
+      "phi" ∷ <nobuf> (ϕ s2 v _) ∗
+      (* The new state must be greater than the possible current states. *)
+      "greater" ∷ (∀ s' v', ⌜ s1 ⊑ s' ⌝ ∗ ϕ s' v' _ -∗ ⌜ s' ⊑ s2 ⌝)
+    }}}
+      #ℓ <-{rel} v @ positive; E
+    {{{ RET #();
+      know_store_lb ℓ s2
+    }}}.
+  Proof.
+    intros Φ. iStartProof (iProp _). iIntros (TV). iNamed 1.
+
+    iNamed "knowProt".
+    iNamed "storeLB".
+    (* We unfold the WP. *)
+    iIntros (TV' incl) "Φpost".
+    rewrite wp_eq /wp_def wpc_eq.
+    iIntros ([[SV PV] BV] incl2) "#val".
+    iApply program_logic.crash_weakestpre.wpc_atomic_no_mask.
+    iSplit; first done.
+
+    iApply wp_extra_state_interp_fupd. { done. }
+    { (* Try and simplify this with lemmas/automation. *)
+      clear.
+      intros ??????? [Ki [??] [??] ? ? step].
+      subst.
+      simpl in *.
+      induction Ki using rev_ind.
+      { simpl in *. subst. inv_impure_thread_step; try done.
+        rewrite list_fmap_singleton.
+        subst.
+        congruence. }
+      move: H.
+      rewrite fill_app.
+      simpl.
+      destruct x; try done.
+      - simpl.
+        rewrite /thread_fill_item.
+        simpl.
+        inversion 1.
+        simpl in *.
+        rewrite -nvm_fill_fill in H2.
+        simpl in *.
+        destruct Ki using rev_ind; try done.
+        { simpl in *. subst. inv_impure_thread_step; try done. }
+        simpl in *.
+        rewrite fill_app in H2.
+        simpl in *.
+        destruct x; try done.
+      - simpl.
+        rewrite /thread_fill_item.
+        simpl.
+        inversion 1.
+        simpl in *.
+        rewrite -nvm_fill_fill in H3.
+        simpl in *.
+        destruct Ki using rev_ind; try done.
+        { simpl in *. subst. inv_impure_thread_step; try done. }
+        simpl in *.
+        rewrite fill_app in H3.
+        simpl in *.
+        destruct x; try done. }
+
+    iNamed 1.
+
+    (* _Before_ we load the points-to predicate we deal with the predicate ϕ. We
+    do this before such that the later that arrises is stripped off when we take
+    the step. *)
+    iDestruct (own_all_preds_pred with "predicates knowPred")
+      as (pred predsLook) "#predsEquiv".
+    
+    (* We need to get the points-to predicate for [ℓ] which is is inside
+    [interp].  We want to look up the points-to predicate in [ptsMap]. To this
+    end, we combine our fragment of the history with the authorative element. *)
+    iDestruct (
+        own_frag_history_agree_singleton with "history knowFragHist") as %look.
+    destruct look as (absHist & enc & absHistLook & lookTS & decodeEnc).
+
+    iDestruct (
+        location_sets_singleton_included with "sharedLocs isSharedLoc"
+      ) as %ℓSh.
+    iDestruct (big_sepM_lookup_acc with "predsHold") as "[predMap predsHold]".
+    { done. }
+    iDestruct "predMap" as
+        (pred' physHist physHistLook predsLook') "predMap".
+    assert (pred = pred') as <-. { apply (inj Some). rewrite -predsLook. done. }
+    clear predsLook'.
+
+    (* We can now get the points-to predicate and execute the load. *)
+    iDestruct (big_sepM_lookup_acc with "ptsMap") as "[pts ptsMap]"; first done.
+
+    iApply (wp_store_release (extra := {| extra_state_interp := True |})
+             with "[$pts $val]").
+    iIntros "!>" (t') "(%look & %gt & #val' & pts)".
+    
+  Qed.
+
+End wp_at_rules.
